Changed some naming conventions, still need to change QProp

src/Checker.v
@@ -58,167 +58,167 @@ Record QProp : Type :=
       unProp : Rose Result
     }.
 
-Definition Property (Gen: Type -> Type) : Type := Gen QProp.
+Definition Checker (Gen: Type -> Type) : Type := Gen QProp.
 
-Section Property.
+Section Checkers.
   Context {Gen : Type -> Type}
           {H: GenMonad Gen}.
 
-  Class Testable (A : Type) : Type :=
+  Class Checkable (A : Type) : Type :=
     {
-      property : A -> Property Gen
+      checker : A -> Checker Gen
     }.
 
   (* mapping and lifting functions *)
-
+  
   Definition liftBool (b : bool) : Result :=
     if b then succeeded else updReason failed "Falsifiable".
 
-  Definition mapProp {P : Type} {_ : Testable P}
-             (f : QProp -> QProp) (prop : P) : Property Gen :=
-    fmapGen f (property prop).
+  Definition mapProp {P : Type} {_ : Checkable P}
+             (f : QProp -> QProp) (prop : P) : Checker Gen :=
+    fmapGen f (checker prop).
 
-  Definition mapRoseResult {P : Type} {_ : Testable P}
-             (f : Rose Result -> Rose Result) (prop : P) : Property Gen :=
+  Definition mapRoseResult {P : Type} {_ : Checkable P}
+             (f : Rose Result -> Rose Result) (prop : P) : Checker Gen :=
     mapProp (fun p => match p with MkProp t => MkProp (f t) end) prop.
 
-  Definition mapTotalResult {prop : Type} {_ : Testable prop}
-             (f : Result -> Result) : prop -> Property Gen :=
+  Definition mapTotalResult {prop : Type} {_ : Checkable prop}
+             (f : Result -> Result) : prop -> Checker Gen :=
     mapRoseResult (fmapRose f).
 
-  (* Testable Instances *)
-  Global Instance testResult : Testable Result :=
+  (* Checkable Instances *)
+  Global Instance testResult : Checkable Result :=
     {|
       (* Left a protectResults out! *)
-      property r := returnGen (MkProp (returnRose r))
+      checker r := returnGen (MkProp (returnRose r))
     |}.
   
 
-  Global Instance testBool : Testable bool :=
+  Global Instance testBool : Checkable bool :=
     {|
-      property b := property (liftBool b)
+      checker b := checker (liftBool b)
     |}.
   
   (* ZP/CH: what's the relation between unit and discards? *)
-  Global Instance testUnit : Testable unit :=
+  Global Instance testUnit : Checkable unit :=
     {|
-      property := fun _ => property rejected
+      checker := fun _ => checker rejected
     |}.
 
-  Global Instance testProp : Testable QProp :=
+  Global Instance testProp : Checkable QProp :=
     {|
-      property p := returnGen p
+      checker p := returnGen p
     |}.
 
-  Global Instance testGenProp (P : Type) : Testable P -> Testable (Gen P) :=
+  Global Instance testGenProp (P : Type) : Checkable P -> Checkable (Gen P) :=
     {|
-      property p := bindGen p property
+      checker p := bindGen p checker
     |}.
 
   
-  (* Property Combinators *)
+  (* Checker Combinators *)
   
   (* The following function on its own does not have a decreasing argument...
 
-     Fixpoint props {prop A : Type} {t : Testable prop}
+     Fixpoint props {prop A : Type} {t : Checkable prop}
                     (pf : A -> prop) (shrinker : A -> list A) (x : A) :=
-       MkRose (property (pf x)) (List.map (props pf shrinker) (shrinker x)).
+       MkRose (checker (pf x)) (List.map (props pf shrinker) (shrinker x)).
    *)
-  Fixpoint props' {prop A : Type} {t : Testable prop} (n : nat)
+  Fixpoint props' {prop A : Type} {t : Checkable prop} (n : nat)
            (pf : A -> prop) (shrinker : A -> list A) (x : A) :=
     match n with
       | O =>
-        MkRose (property (pf x)) (lazy nil)
+        MkRose (checker (pf x)) (lazy nil)
       | S n' =>
-        MkRose (property (pf x)) (lazy (List.map (props' n' pf shrinker) (shrinker x)))
+        MkRose (checker (pf x)) (lazy (List.map (props' n' pf shrinker) (shrinker x)))
     end.
 
   (* Arbitrary choice for number of shrinks.. *)
-  Definition props {prop A : Type} `{Testable prop}
-             (pf : A -> prop) (shrinker : A -> list A) (x : A) : Rose (Property Gen) :=
+  Definition props {prop A : Type} `{Checkable prop}
+             (pf : A -> prop) (shrinker : A -> list A) (x : A) : Rose (Checker Gen) :=
     props' 1000 pf shrinker x.
 
-  Definition shrinking {prop A : Type} `{Testable prop}
-             (shrinker : A -> list A) (x0 : A) (pf : A -> prop) : Property Gen :=
+  Definition shrinking {prop A : Type} `{Checkable prop}
+             (shrinker : A -> list A) (x0 : A) (pf : A -> prop) : Checker Gen :=
     @fmapGen Gen _ _ _ (fun x => MkProp (joinRose (fmapRose unProp x)))
              (promote (props pf shrinker x0)).
 
-  Definition callback {prop : Type} `{Testable prop}
-             (cb : Callback) : prop -> Property Gen :=
+  Definition callback {prop : Type} `{Checkable prop}
+             (cb : Callback) : prop -> Checker Gen :=
     mapTotalResult (fun r => addCallback r cb).
 
-  Definition printTestCase {prop : Type} `{Testable prop}
-             (s : string) (p : prop) : Property Gen :=
+  Definition printTestCase {prop : Type} `{Checkable prop}
+             (s : string) (p : prop) : Checker Gen :=
     callback (PostFinalFailure Counterexample (fun _st _res => trace s 0)) p.
 
-  Definition whenFail {prop : Type} `{Testable prop}
-             (str : string) : prop -> Property Gen :=
+  Definition whenFail {prop : Type} `{Checkable prop}
+             (str : string) : prop -> Checker Gen :=
     callback (PostFinalFailure Counterexample (fun _st _sr => trace str 0)).
 
 
-  Definition expectFailure {prop: Type} `{Testable prop} (p: prop) := 
+  Definition expectFailure {prop: Type} `{Checkable prop} (p: prop) := 
     mapTotalResult (fun res =>
                       MkResult (ok res) false (reason res) 
                              (interrupted res) (stamp res) (callbacks res))
                    p.
 
-  Definition cover {prop : Type} {_ : Testable prop}
-             (b : bool) (n : nat) (s : string) : prop -> Property Gen :=
+  Definition cover {prop : Type} {_ : Checkable prop}
+             (b : bool) (n : nat) (s : string) : prop -> Checker Gen :=
     if b then
       mapTotalResult (fun res =>
                         let '(MkResult o e r i st c) := res in
                         MkResult o e r i ((s,n)::st) c)
-    else property.
+    else checker.
 
-  Definition classify {prop : Type} {_ : Testable prop}
-             (b : bool) (s : string) : prop -> Property Gen :=
+  Definition classify {prop : Type} {_ : Checkable prop}
+             (b : bool) (s : string) : prop -> Checker Gen :=
     cover b 0 s.
 
-  Definition label {prop : Type} {_ : Testable prop}
-             (s : string) : prop -> Property Gen :=
+  Definition label {prop : Type} {_ : Checkable prop}
+             (s : string) : prop -> Checker Gen :=
     classify true s.
 
-  Definition collect {A prop : Type} `{_ : Show A} {_ : Testable prop}
-             (x : A) : prop -> Property Gen :=
+  Definition collect {A prop : Type} `{_ : Show A} {_ : Checkable prop}
+             (x : A) : prop -> Checker Gen :=
     label (show x).
 
 
-  Definition implication {prop : Type} `{Testable prop} (b : bool) (p : prop) :=
-    if b then property p else property rejected.
+  Definition implication {prop : Type} `{Checkable prop} (b : bool) (p : prop) :=
+    if b then checker p else checker rejected.
        
 
-  Definition forAll {A prop : Type} {_ : Testable prop} `{Show A}
-             (gen : Gen A)  (pf : A -> prop) : Property Gen :=
+  Definition forAll {A prop : Type} {_ : Checkable prop} `{Show A}
+             (gen : Gen A)  (pf : A -> prop) : Checker Gen :=
     bindGen gen (fun x =>
     printTestCase (show x ++ newline) (pf x)).
 
-   Definition forAllShrink {A prop : Type} {_ : Testable prop} `{Show A}
-              (gen : Gen A) (shrinker : A -> list A) (pf : A -> prop) : Property Gen :=
+   Definition forAllShrink {A prop : Type} {_ : Checkable prop} `{Show A}
+              (gen : Gen A) (shrinker : A -> list A) (pf : A -> prop) : Checker Gen :=
      bindGen gen (fun x =>
      shrinking shrinker x (fun x' =>
      printTestCase (show x' ++ newline) (pf x'))).
 
   Global Instance testFun {A prop : Type} `{Show A}
-         {_ : Arbitrary A} {_ : Testable prop} : Testable (A -> prop) :=
+         {_ : Arbitrary A} {_ : Checkable prop} : Checkable (A -> prop) :=
     {
-      property f := forAllShrink arbitrary shrink f
+      checker f := forAllShrink arbitrary shrink f
     }.
 
-  Global Instance testPolyFun {prop : Type -> Type} {_ : Testable (prop nat)} : Testable (forall T, prop T) :=
+  Global Instance testPolyFun {prop : Type -> Type} {_ : Checkable (prop nat)} : Checkable (forall T, prop T) :=
     {
-      property f := printTestCase "" (f nat)
+      checker f := printTestCase "" (f nat)
     }.
 
-  Global Instance testPolyFunSet {prop : Set -> Type} {_ : Testable (prop nat)} : Testable (forall T, prop T) :=
+  Global Instance testPolyFunSet {prop : Set -> Type} {_ : Checkable (prop nat)} : Checkable (forall T, prop T) :=
     {
-      property f := printTestCase "" (f nat)
+      checker f := printTestCase "" (f nat)
     }.
 
 
-End Property.
+End Checkers.
 
 Notation "x ==> y" := (implication x y) (at level 55, right associativity) 
-                      : Property_scope.
+                      : Checker_scope.
 
 
  
