src/EndToEnd.v
@@ -3,7 +3,7 @@ Require Import AbstractGen SetOfOutcomes Arbitrary Property.
 Require Import ssreflect ssrbool eqtype.
 
  
-Definition Property := Property Pred.
+Definition Checker := Checker Pred.
 
 Definition resultSuccessful (r : Result) : bool :=
   match r with
@@ -17,22 +17,22 @@ Definition success qp :=
     | MkProp (MkRose res _) => resultSuccessful res
   end.
 
-(* Maps a Property to a Prop *)
-Definition semProperty (P : Property) : Prop :=
+(* Maps a Checker to a Prop *)
+Definition semChecker (P : Checker) : Prop :=
   forall qp, P qp -> success qp = true.
 
-(* Maps a Testable to a Prop i.e. gives an equivalent proposition to the
+(* Maps a Checkable to a Prop i.e. gives an equivalent proposition to the
    property under test *)
-Definition semTestable {A : Type} {_ : Testable  A} (a : A) : Prop :=
-  semProperty (property a).
+Definition semCheckable {A : Type} {_ : Checkable  A} (a : A) : Prop :=
+  semChecker (checker a).
 
 Lemma mapTotalResult_id:
-  forall {prop : Type} {H : Testable prop} (f : Result -> Result) (p : prop),
+  forall {prop : Type} {H : Checkable prop} (f : Result -> Result) (p : prop),
     (forall res, resultSuccessful res = resultSuccessful (f res)) ->
-    (semProperty (mapTotalResult f p) <-> semTestable p).
+    (semChecker (mapTotalResult f p) <-> semCheckable p).
 Proof.
   move => prop H f p Hyp.
-  rewrite /semTestable  /mapTotalResult /mapRoseResult /mapProp /semProperty.
+  rewrite /semCheckable  /mapTotalResult /mapRoseResult /mapProp /semChecker.
   split.
   - move=> H1 qp Hprop.
     rewrite fmapGen_def in H1.
@@ -49,8 +49,8 @@ Proof.
 Qed.
 
 Lemma semCallback_id:
-  forall {prop : Type} {H : Testable prop} (cb : Callback) (p : prop),
-    semProperty (callback cb p) <-> semTestable p.
+  forall {prop : Type} {H : Checkable prop} (cb : Callback) (p : prop),
+    semChecker (callback cb p) <-> semCheckable p.
 Proof.
   move => prop tp cb p. rewrite /callback.
   split; move => H.
@@ -61,36 +61,36 @@ Proof.
 Qed.
 
 Lemma semWhenFail_id:
-  forall {prop : Type} {H : Testable prop} (s : String.string) (p : prop),
-    semProperty (whenFail s p) <-> semTestable p.
+  forall {prop : Type} {H : Checkable prop} (s : String.string) (p : prop),
+    semChecker (whenFail s p) <-> semCheckable p.
 Proof.
   move => prop H s p. by rewrite /whenFail semCallback_id.
 Qed.
 
 
 Lemma semPrintTestCase_id:
-  forall {prop: Type} {tp : Testable prop} (s: String.string) (p: prop),
-    semProperty (printTestCase s p) <-> semTestable p.
+  forall {prop: Type} {tp : Checkable prop} (s: String.string) (p: prop),
+    semChecker (printTestCase s p) <-> semCheckable p.
 Proof.
   move => prop tp s p. by rewrite /printTestCase semCallback_id.
 Qed.
 
 Lemma semShrinking_id_aux:
-  forall {prop A : Type} {H : Testable prop}
+  forall {prop A : Type} {H : Checkable prop}
          (shrinker : A -> list A) (x0 : A) (pf : A -> prop) n,
-    semProperty (fmapGen (fun x => MkProp (joinRose (fmapRose unProp x)))
+    semChecker (fmapGen (fun x => MkProp (joinRose (fmapRose unProp x)))
                          (promote ((props' n pf shrinker x0)))) <->
-    semTestable (pf x0).
+    semCheckable (pf x0).
 Proof.
   move=> prop A H shrinker x0 pf n. destruct n.
-  -  rewrite /semTestable /semProperty !fmapGen_def. split.
+  -  rewrite /semCheckable /semChecker !fmapGen_def. split.
      + move => Hfail qp Hprop. apply Hfail. eexists.
        split. rewrite /promote /PredMonad /promoteP /=.
        exists qp. split => //. by destruct qp as [[[] []]].
      + move=> Hfail qp [rqp  [[qp' [Hprop Heq']] Heq]].
        rewrite /returnP in Heq'; subst. apply Hfail.
        by destruct qp' as [[[] []]].
-  - rewrite /semTestable fmapGen_def /semProperty /= /bindP /returnP /=.
+  - rewrite /semCheckable fmapGen_def /semChecker /= /bindP /returnP /=.
     split.
     + move=> Hfail qp Hprop. apply Hfail. eexists.
       split. exists qp. split => //. by destruct qp as [[[] []]].
@@ -99,19 +99,19 @@ Proof.
 Qed.
 
 Lemma semShrinking_id:
-  forall {prop A : Type} {H : Testable prop}
+  forall {prop A : Type} {H : Checkable prop}
          (shrinker : A -> list A) (x0 : A) (pf : A -> prop),
-    semProperty (shrinking shrinker x0 pf) <->
-    semTestable (pf x0).
+    semChecker (shrinking shrinker x0 pf) <->
+    semCheckable (pf x0).
 Proof.
   move=> prop A H shrinker x0 pf.
   rewrite /shrinking /props. apply semShrinking_id_aux.
 Qed.
 
 Lemma semCover_id:
-  forall {prop : Type} {H : Testable prop} (b: bool) (n: nat)
+  forall {prop : Type} {H : Checkable prop} (b: bool) (n: nat)
          (s: String.string) (p : prop),
-    semProperty (cover b n s p) <-> semTestable p.
+    semChecker (cover b n s p) <-> semCheckable p.
 Proof.
   move=> prop H b n s p. split.
   - rewrite /cover. case: b => //.
@@ -123,40 +123,40 @@ Proof.
 Qed.
 
 Lemma semClassify_id:
-   forall {prop : Type} {H : Testable prop} (b: bool) (s: String.string)
+   forall {prop : Type} {H : Checkable prop} (b: bool) (s: String.string)
           (p : prop),
-    semProperty (classify b s p) <-> semTestable p.
+    semChecker (classify b s p) <-> semCheckable p.
 Proof.
   move=> prop H b s p. by rewrite /classify semCover_id.
 Qed.
 
 Lemma semLabel_id:
-   forall {prop : Type} {H : Testable prop} (s: String.string)
+   forall {prop : Type} {H : Checkable prop} (s: String.string)
           (p : prop),
-    semProperty (label s p) <-> semTestable p.
+    semChecker (label s p) <-> semCheckable p.
 Proof.
   move=> prop H s p. by rewrite /label semClassify_id.
 Qed.
 
 Lemma semCollect_id:
-   forall {prop : Type} {H : Testable prop} (s: String.string)
+   forall {prop : Type} {H : Checkable prop} (s: String.string)
           (p : prop),
-    semProperty (collect s p) <-> semTestable p.
+    semChecker (collect s p) <-> semCheckable p.
 Proof.
   move=> prop H s p. by rewrite /collect semLabel_id.
 Qed.
 
-Open Scope Property_scope.
+Open Scope Checker_scope.
 
 Lemma semImplication:
-      forall {prop : Type} {H : Testable prop}
+      forall {prop : Type} {H : Checkable prop}
              (p : prop) (b : bool),
-        semProperty (b ==> p) <-> b = true -> semTestable p.
+        semChecker (b ==> p) <-> b = true -> semCheckable p.
 Proof.
   move => prop H p b. case: b.
   - split => /=; auto. apply. reflexivity.
   - split; try congruence. move => _.
-    rewrite /implication.  rewrite /semProperty /property /testResult.
+    rewrite /implication.  rewrite /semChecker /checker /testResult.
     move => qp. rewrite returnGen_def. by move => <-.
 Qed.
   
@@ -164,10 +164,10 @@ Qed.
 (* equivalences for other combinators *)
 
 Lemma semBindGen:
-  forall {A } (gen : Pred A) (p : A -> Property),
-    semProperty (bindGen gen p) <-> forall g, gen g -> semProperty (p g).
+  forall {A } (gen : Pred A) (p : A -> Checker),
+    semChecker (bindGen gen p) <-> forall g, gen g -> semChecker (p g).
 Proof.
-  move=> A gen prop. rewrite /semProperty. split.
+  move=> A gen prop. rewrite /semChecker. split.
   - move => H g Hgen qp Hprop. apply H.  
     eexists. split; eassumption. 
   - move => H qp [a [Hgen Hprop]]. eauto.
@@ -175,29 +175,29 @@ Qed.
 
 Lemma semReturnGen:
   forall (p : QProp),
-    semProperty (returnGen p) <-> semTestable p.
+    semChecker (returnGen p) <-> semCheckable p.
 Proof.
-  move=> p. rewrite /semProperty. split;
+  move=> p. rewrite /semChecker. split;
   move => H qp Hprop; auto.
 Qed.
 
 Lemma semPredQProp:
-  forall (p : Pred QProp), semTestable p <-> (semProperty p).
+  forall (p : Pred QProp), semCheckable p <-> (semChecker p).
 Proof.
    move=> p.
-  rewrite /semTestable /property /testGenProp /property /testProp semBindGen.
+  rewrite /semCheckable /checker /testGenProp /checker /testProp semBindGen.
   split.
-  - move => H pq /H Hgen. rewrite returnGen_def /semProperty in Hgen.
+  - move => H pq /H Hgen. rewrite returnGen_def /semChecker in Hgen.
     by apply Hgen.
-  - move => H pq Hgen. rewrite returnGen_def /semProperty.
-    move => qp Heq; subst. rewrite /semProperty in H. by auto.
+  - move => H pq Hgen. rewrite returnGen_def /semChecker.
+    move => qp Heq; subst. rewrite /semChecker in H. by auto.
 Qed.
 
 Lemma semForAll :
-  forall {A prop : Type} {H : Testable prop} `{Show A} 
+  forall {A prop : Type} {H : Checkable prop} `{Show A} 
          (gen : Pred A) (f : A -> prop),
-    semProperty (forAll gen f) <->
-    forall a : A, gen a -> semTestable (f a).
+    semChecker (forAll gen f) <->
+    forall a : A, gen a -> semCheckable (f a).
 Proof.
   move => A prop Htest show gen pf. split => H'.
   - rewrite /forAll in H'. move/semBindGen : H' => H' a /H' Hgen.
@@ -207,10 +207,10 @@ Proof.
 Qed.
 
 Lemma semForAllShrink:
-  forall {A prop : Type} {H : Testable prop} `{Show A}
+  forall {A prop : Type} {H : Checkable prop} `{Show A}
          (gen : Pred A) (f : A -> prop) shrinker,
-    semProperty (forAllShrink gen shrinker f) <->
-    forall a : A, gen a -> semTestable (f a).
+    semChecker (forAllShrink gen shrinker f) <->
+    forall a : A, gen a -> semCheckable (f a).
 Proof.
   move => A prop H show gen pf shrink. split.
   - rewrite /forAllShrink semBindGen.
@@ -222,23 +222,23 @@ Proof.
     rewrite semPrintTestCase_id. by auto.
 Qed.
 
-(* equivalent Props for Testables *)
+(* equivalent Props for Checkables *)
 
 Lemma semBool:
-  forall (b : bool), semTestable b <-> b = true.
+  forall (b : bool), semCheckable b <-> b = true.
 Proof.  
   move => b. case: b.
   - split => //. compute.
     by move => _ qp Heq; subst.
-  - split => //. rewrite /semTestable /semProperty. move => H.
+  - split => //. rewrite /semCheckable /semChecker. move => H.
     simpl in H.  rewrite /returnP /= in H. 
     by specialize (H _ Logic.eq_refl).
 Qed.
 
 Lemma semResult:
-  forall (res: Result), semTestable res <-> resultSuccessful res = true.
+  forall (res: Result), semCheckable res <-> resultSuccessful res = true.
 Proof.
-  rewrite /semTestable /property /testResult /semProperty.
+  rewrite /semCheckable /checker /testResult /semChecker.
   move => res. split.
   + move=> /(_ ({| unProp := returnRose res |})) /= H.
     by apply H.
@@ -246,16 +246,16 @@ Proof.
 Qed.
 
 Lemma semUnit:
-  forall (t: unit), semTestable t <-> True.
+  forall (t: unit), semCheckable t <-> True.
 Proof.
   move => t. split => // _. compute.
   by move => qp Heq; subst.
 Qed.
 
 Lemma semQProp:
-  forall (qp: QProp), semTestable qp <-> success qp = true.
+  forall (qp: QProp), semCheckable qp <-> success qp = true.
 Proof.
-  move => qp. rewrite /semTestable /semProperty /property
+  move => qp. rewrite /semCheckable /semChecker /checker
                       /testProp returnGen_def.
   split.
   - auto.
@@ -263,55 +263,55 @@ Proof.
 Qed.
 
 Lemma semGen:
-  forall (P : Type) {H : Testable P} (gen: Pred P),
-    (semTestable gen) <-> (forall p, gen p -> semTestable p).
+  forall (P : Type) {H : Checkable P} (gen: Pred P),
+    (semCheckable gen) <-> (forall p, gen p -> semCheckable p).
 Proof.
   move=> P H gen. split.
-  - move=> Hsem qp Hgen. rewrite /semTestable /semProperty in Hsem *.
-    move => qp' Hprop. apply Hsem. rewrite /property /testGenProp bindGen_def.
+  - move=> Hsem qp Hgen. rewrite /semCheckable /semChecker in Hsem *.
+    move => qp' Hprop. apply Hsem. rewrite /checker /testGenProp bindGen_def.
     exists qp. split => //.
-  - move => H'. rewrite /semTestable /semProperty. move=> qp prop.
-    rewrite /property /testGenProp in prop. move : prop => [p [/H' Hgen Hprop]].
-    rewrite /semTestable /semProperty in Hgen. by auto.
+  - move => H'. rewrite /semCheckable /semChecker. move=> qp prop.
+    rewrite /checker /testGenProp in prop. move : prop => [p [/H' Hgen Hprop]].
+    rewrite /semCheckable /semChecker in Hgen. by auto.
 Qed.
 
 Lemma semFun:
-  forall {A prop : Type} {H1 : Show A} {H2 : Arbitrary A} {H3 : Testable prop}
+  forall {A prop : Type} {H1 : Show A} {H2 : Arbitrary A} {H3 : Checkable prop}
          (f : A -> prop),
-    semTestable f <->
-    forall (a : A), (arbitrary : Pred A) a -> semTestable (f a).
+    semCheckable f <->
+    forall (a : A), (arbitrary : Pred A) a -> semCheckable (f a).
 Proof.
   move=> A prop H1 H2 H3 f.
-  rewrite /semTestable /property /testFun.
+  rewrite /semCheckable /checker /testFun.
   split.
   - move => /semForAllShrink H' a' /H' Gen. by auto.
   - move => H'. apply semForAllShrink => a' /H' Hgen. by auto.
 Qed.
 
-(* I think this is the strongest property we can get for polymorphic functions *)
+(* I think this is the strongest checker we can get for polymorphic functions *)
 Lemma semPolyFun:
-  forall {prop : Type -> Type} {H : Testable (prop nat)} (f : forall T, prop T),
-    (semTestable f) <-> (semTestable (f nat)).
+  forall {prop : Type -> Type} {H : Checkable (prop nat)} (f : forall T, prop T),
+    (semCheckable f) <-> (semCheckable (f nat)).
 Proof.
-  move => prop H f. rewrite /semTestable {2}/property /testPolyFun.
+  move => prop H f. rewrite /semCheckable {2}/checker /testPolyFun.
   by rewrite semPrintTestCase_id.
 Qed.
 
 Lemma semPolyFunSet:
-  forall {prop : Set -> Type} {H : Testable (prop nat)} (f : forall T, prop T),
-    (semTestable f) <->  (semTestable (f nat)).
+  forall {prop : Set -> Type} {H : Checkable (prop nat)} (f : forall T, prop T),
+    (semCheckable f) <->  (semCheckable (f nat)).
 Proof.
-  move => prop H f. rewrite /semTestable {2}/property /testPolyFun.
+  move => prop H f. rewrite /semCheckable {2}/checker /testPolyFun.
   by rewrite semPrintTestCase_id.
 Qed.
 
 (* A typeclass so we can automate the application of the previous theorems
   and get a readable Prop *)
 
-Class Provable (A : Type) {H: Testable A} : Type :=
+Class Provable (A : Type) {H: Checkable A} : Type :=
  {
     proposition : A -> Prop;
-    _ : forall a, proposition a <-> semTestable a
+    _ : forall a, proposition a <-> semCheckable a
   }.
 
 Program Instance proveResult : Provable Result :=
